Phi_Test/PhiTest_Mem_C.thy
@@ -112,17 +112,15 @@ proc test_mem8:
     $addr \<tribullet> d \<tribullet> e := \<open>2 \<Ztypecolon> \<nat>\<close>
   \<medium_right_bracket> .
 
-proc test_mem8a:
-  input  \<open>(x,(y,z)) \<Ztypecolon> \<m>\<e>\<m>[addr] \<lbrace> c: \<nat>, d: \<lbrace> b: \<nat>, e: \<nat>\<rbrace> \<rbrace>\<heavy_comma> addr \<Ztypecolon> \<v>\<a>\<l> \<Pp>\<t>\<r> \<s>\<t>\<r>\<u>\<c>\<t> {c: \<a>\<i>\<n>\<t>, d: \<s>\<t>\<r>\<u>\<c>\<t> {b: \<a>\<i>\<n>\<t>, e: \<a>\<i>\<n>\<t>}}\<close>
-  output \<open>(x,(y,2)) \<Ztypecolon> \<m>\<e>\<m>[addr] \<lbrace> c: \<nat>, d: \<lbrace> b: \<nat>, e: \<nat>\<rbrace> \<rbrace>\<close>
-  \<medium_left_bracket> note [[\<phi>trace_reasoning = 2]] 
-    ;; \<open>2 \<Ztypecolon> \<nat>\<close>
-    
-    ;;
-    \<open>(2,3) \<Ztypecolon> \<lbrace> b: \<nat>, e: \<nat>\<rbrace>\<close>
-
-
 declare [[\<phi>reasoning_step_limit = 140]]
+
+proc test_mem8a:
+  input  \<open>(x,y,z) \<Ztypecolon> \<m>\<e>\<m>[addr] \<lbrace> c: \<nat>, d: \<lbrace> b: \<nat>, e: \<nat>\<rbrace> \<rbrace>\<heavy_comma> addr \<Ztypecolon> \<v>\<a>\<l> \<Pp>\<t>\<r> \<s>\<t>\<r>\<u>\<c>\<t> {c: \<a>\<i>\<n>\<t>, d: \<s>\<t>\<r>\<u>\<c>\<t> {b: \<a>\<i>\<n>\<t>, e: \<a>\<i>\<n>\<t>}}\<close>
+  output \<open>(x,2,3) \<Ztypecolon> \<m>\<e>\<m>[addr] \<lbrace> c: \<nat>, d: \<lbrace> b: \<nat>, e: \<nat>\<rbrace> \<rbrace>\<close>
+  \<medium_left_bracket>
+    $addr \<tribullet> d := \<open>(2,3) \<Ztypecolon> \<lbrace> b: \<nat>, e: \<nat>\<rbrace>\<close>
+  \<medium_right_bracket> .
+
 
 proc test_mem9:
   input  \<open>(x,(y,z,(g,h,i,j))) \<Ztypecolon> \<m>\<e>\<m>[addr] \<lbrace> c: \<nat>, d: \<lbrace> b: \<nat>, e: \<nat>, f: \<lbrace> g: \<nat>, h: \<nat>, i: \<nat>, j: \<nat> \<rbrace> \<rbrace> \<rbrace>\<heavy_comma>
